1) pick any node u
2) find the node which is farthest from u, call it x (calculate using the same approach as in Solution 1)
3) find the node which is farthest from x, call it q (calculate using the same approach as in Solution 1)
The answer will be the length of a path from x to q.

Proof of correctness:

The crucial step is to prove that x will be one of the endpoints of the path with maximal length (note that there might be more than one such path). If it is, then the longest path from x will be the longest path in the tree.

Let d(v1, v2) be length of path between v1 and v2

Letâ€™s prove it by contradiction: assume there is a strictly longer path between s and t, neither of which is x. Let h be a node which is closest to u among the nodes on a path between s and t. Then there are two cases:
1) h is on path between u and x

    u
    |
    |
    |
    h   x
   / \ /
  /   *
 /     \
s       t 
then d(s, t) = d(s, h) + d(h, t) <= d(s, h) + d(h, x) = d(s, x), which contradicts assumption.

2) h is not on path between u and x

    u
    |
    *---x
    |
    h
   / \
  /   \
 /     \
s       t
then

d(u, s) <= d(u, x) <= d(u, h) + d(h, x)
d(u, t) <= d(u, x) <= d(u, h) + d(h, x)

d(s, t) = d(s, h) + d(h, t)
= d(u, s) + d(u, t) - 2 d(u, h)
<= 2 d(h, x)

2 d(s, t) <= d(s, t) + 2 d(h, x)
= d(s, h) + d(h, x) + d(x, h) + d(h, t)
= d(x, s) + d(x, t)

This means that max(d(v, s), d(v, t)) >= d(s, t), which also contradicts assumption.

Thus, we proved that farthest node of a node will be one of the endpoints of the longest path.
